@prefix : <https://gallosiciliani.unict.it/ns/liph#> .
@prefix owl: <http://www.w3.org/2002/07/owl#> .
@prefix rdf: <http://www.w3.org/1999/02/22-rdf-syntax-ns#> .
@prefix xml: <http://www.w3.org/XML/1998/namespace> .
@prefix xsd: <http://www.w3.org/2001/XMLSchema#> .
@prefix rdfs: <http://www.w3.org/2000/01/rdf-schema#> .
@prefix vann: <http://purl.org/vocab/vann/> .
@prefix eurio: <http://data.europa.eu/s66#> .
@prefix dcterms: <http://purl.org/dc/terms/> .
@prefix ontolex: <https://www.w3.org/ns/lemon/ontolex#> .
@base <https://gallosiciliani.unict.it/ns/liph#> .

<https://gallosiciliani.unict.it/ns/liph> rdf:type owl:Ontology ;
                                           owl:versionIRI <https://gallosiciliani.unict.it/ns/liph/2.0.0> ;
                                           owl:imports <http://data.europa.eu/s66/v2.4#> ,
                                                       <http://www.w3.org/ns/lemon/ontolex> ;
                                           dcterms:contributor "Daniele Francesco Santamaria" ,
                                                               "Domenico Cantone" ,
                                                               "Marianna Nicolosi Asmundo" ,
                                                               "Salvatore Menza" ,
                                                               "Vincenzo Nicolò Di Caro" ;
                                           dcterms:created "2024-08-08"^^xsd:date ;
                                           dcterms:creator "Cristiano Longo" ;
                                           dcterms:description """The Linguistic Phenomena Ontology is an Ontolex-lemon extension devoted to represent linguistic phenomena.  We denote as linguistic phenomena those kinds of phenomena which cause modifications of language expressions. In general, a linguistic phenomenon occurs by turning a parent expression into a target expression in the language under consideration, where the parent expression may have been inherited from the parent language, or it may have been borrowed from a foreign language.

In addition, the ontology provides the regex and replacement properties to describe a linguistic phenomenon operatioanally in a machine-actionable way.

This work has been created in the scope of the project PRIN 2022 PNRR “Contact-induced change and sociolinguistics: an experimental study on the Gallo-Italic dialects of Sicily\", founded by the European Union – Next Generation EU, Mission 4, Component 1, CUP J53D23017360001 - ID P2022YWS8T."""@en ;
                                           dcterms:license <https://creativecommons.org/licenses/by/4.0/> ;
                                           dcterms:modified "2024-11-19"^^xsd:date ;
                                           dcterms:title "The Linguistic Phenomena Ontology (LiPh)"@en ;
                                           vann:preferredNamespacePrefix "liph" ;
                                           vann:preferredNamespaceUri "https://gallosiciliani.unict.it/ns/liph#" ;
                                           rdfs:comment """The Linguistic Phenomena Ontology is an Ontolex-lemon extension devoted to represent linguistic phenomena.  We denote as linguistic phenomena those kinds of phenomena which cause modifications of language expressions. In general, a linguistic phenomenon occurs by turning a parent expression into a target expression in the language under consideration, where the parent expression may have been inherited from the parent language, or it may have been borrowed from a foreign language.

In addition, the ontology provides the regex and replacement properties to describe a linguistic phenomenon operatioanally in a machine-actionable way."""@en ;
                                           rdfs:label "The Linguistic Phenomena Ontology (LiPh)"@en ;
                                           owl:priorVersion "1.2.0" ;
                                           owl:versionInfo "2.0.0" .

#################################################################
#    Annotation properties
#################################################################

###  http://data.europa.eu/s66#isResultOf
eurio:isResultOf rdf:type owl:AnnotationProperty .


###  http://purl.org/dc/terms/contributor
dcterms:contributor rdf:type owl:AnnotationProperty .


###  http://purl.org/dc/terms/created
dcterms:created rdf:type owl:AnnotationProperty .


###  http://purl.org/dc/terms/creator
dcterms:creator rdf:type owl:AnnotationProperty .


###  http://purl.org/dc/terms/description
dcterms:description rdf:type owl:AnnotationProperty .


###  http://purl.org/dc/terms/license
dcterms:license rdf:type owl:AnnotationProperty .


###  http://purl.org/dc/terms/title
dcterms:title rdf:type owl:AnnotationProperty .


###  http://purl.org/vocab/vann/preferredNamespacePrefix
vann:preferredNamespacePrefix rdf:type owl:AnnotationProperty .


###  https://gallosiciliani.unict.it/ns/liph#regex
:regex rdf:type owl:AnnotationProperty ;
       rdfs:comment "Used in conjuction with replacement, it allows one to provide an operational description of a linguistic phenomenon. In particular, regex represent the regular expression which recognizes the parts of the parent strings which may be affected by the phenomenon." ;
       rdfs:label "Regular expression pattern" ;
       owl:deprecated "true"^^xsd:boolean ;
       rdfs:range xsd:string ;
       rdfs:domain :linguisticPhenomenon .


###  https://gallosiciliani.unict.it/ns/liph#replacement
:replacement rdf:type owl:AnnotationProperty ;
             rdfs:comment "Used in conjuction with regex, it allows one to provide an operational description of a linguistic phenomenon. In particular, this property define  how parts of the language expression matching the regex have to be replaced. Replacements may contain references to capturing groups defined in regex." ;
             rdfs:label "replacement" ;
             owl:deprecated "true"^^xsd:boolean ;
             rdfs:range xsd:string ;
             rdfs:domain :linguisticPhenomenon .


#################################################################
#    Object Properties
#################################################################

###  https://gallosiciliani.unict.it/ns/liph#derives
:derives rdf:type owl:ObjectProperty ,
                  owl:TransitiveProperty ,
                  owl:ReflexiveProperty ;
         owl:propertyChainAxiom ( [ owl:inverseOf :source
                                  ]
                                  :target
                                ) ;
         rdfs:comment "A derivation is a chain of linguistic phenomena occurrences, may be zero-lenght, which turned the subject lexical expression into the object one." ;
         rdfs:label "derives" .


###  https://gallosiciliani.unict.it/ns/liph#linguisticPhenomenon
:linguisticPhenomenon rdf:type owl:ObjectProperty ,
                               owl:TransitiveProperty ,
                               owl:ReflexiveProperty ;
                      rdfs:comment "An hypothetical change in the morphology or pronunciation of a language expression. Usually, a procedural description of such a phenomenon can be provided (for example \"replace t with d\"). A linguistic phenomenon can generate several resulting expressions, for example if applied to different parts of source ones." ;
                      rdfs:label "linguistic phenomenon" ;
                      owl:deprecated "true"^^xsd:boolean .


###  https://gallosiciliani.unict.it/ns/liph#occurrenceOf
:occurrenceOf rdf:type owl:ObjectProperty ,
                       owl:FunctionalProperty ;
              rdfs:comment "denotes that an individual is an occurrence of a specific linguistic phenomenon" ;
              rdfs:label "is occurrence of" .


###  https://gallosiciliani.unict.it/ns/liph#source
:source rdf:type owl:ObjectProperty ,
                 owl:FunctionalProperty ;
        rdfs:comment "The source lexical object, modified by the linguistic phenomenon" ;
        rdfs:label "source" .


###  https://gallosiciliani.unict.it/ns/liph#target
:target rdf:type owl:ObjectProperty ,
                 owl:FunctionalProperty ;
        rdfs:comment "How a source lexical object has been modified by the linguistic phenomenon" ;
        rdfs:label "target" .


#################################################################
#    Data properties
#################################################################

###  http://www.w3.org/ns/lemon/ontolex#writtenRep
<http://www.w3.org/ns/lemon/ontolex#writtenRep> rdfs:subPropertyOf :writtenRep .


###  https://gallosiciliani.unict.it/ns/liph#matchingPattern
:matchingPattern rdf:type owl:DatatypeProperty ,
                          owl:FunctionalProperty ;
                 rdfs:domain :FiniteStateLinguisticPhenomenon ;
                 rdfs:range xsd:string ;
                 rdfs:comment "A regular expression indicating the parts of a lexical expression which are subject to be replaced" ;
                 rdfs:label "matching pattern" .


###  https://gallosiciliani.unict.it/ns/liph#replaceWith
:replaceWith rdf:type owl:DatatypeProperty ,
                      owl:FunctionalProperty ;
             rdfs:domain :FiniteStateLinguisticPhenomenon ;
             rdfs:range xsd:string ;
             rdfs:comment "How the matched parts of a lexical expression have to be replaced" .


###  https://gallosiciliani.unict.it/ns/liph#writtenRep
:writtenRep rdf:type owl:DatatypeProperty ;
            rdfs:range rdf:langString .


#################################################################
#    Classes
#################################################################

###  http://www.w3.org/ns/lemon/ontolex#Form
<http://www.w3.org/ns/lemon/ontolex#Form> rdfs:subClassOf :LexicalObject .


###  https://gallosiciliani.unict.it/ns/liph#FiniteStateLinguisticPhenomenon
:FiniteStateLinguisticPhenomenon rdf:type owl:Class ;
                                 rdfs:subClassOf :LinguisticPhenomenon ,
                                                 [ rdf:type owl:Restriction ;
                                                   owl:onProperty :matchingPattern ;
                                                   owl:someValuesFrom xsd:string
                                                 ] ,
                                                 [ rdf:type owl:Restriction ;
                                                   owl:onProperty :replaceWith ;
                                                   owl:someValuesFrom xsd:string
                                                 ] ;
                                 rdfs:comment "An executable phenomenon described in terms of regular relations." ;
                                 rdfs:label "Finite-State Linguistic Phenomenon" .


###  https://gallosiciliani.unict.it/ns/liph#LexicalObject
:LexicalObject rdf:type owl:Class ;
               rdfs:subClassOf [ rdf:type owl:Restriction ;
                                 owl:onProperty :derives ;
                                 owl:allValuesFrom :LexicalObject
                               ] ,
                               [ rdf:type owl:Restriction ;
                                 owl:onProperty :writtenRep ;
                                 owl:someValuesFrom rdf:langString
                               ] ;
               owl:disjointWith :LinguisticPhenomenon ,
                                :LinguisticPhenomenonOccurrence ;
               rdfs:comment "A generic object representing a lexical expression involved in some lexical processes is some way." ;
               rdfs:label "lexical object" .


###  https://gallosiciliani.unict.it/ns/liph#LinguisticPhenomenon
:LinguisticPhenomenon rdf:type owl:Class ;
                      owl:disjointWith :LinguisticPhenomenonOccurrence ;
                      rdfs:comment "Instances of this class represent linguistic phenomena, i.e., phenomena that change lexical expressions." ;
                      rdfs:label "Simple Linguistic Phenomenon" .


###  https://gallosiciliani.unict.it/ns/liph#LinguisticPhenomenonOccurrence
:LinguisticPhenomenonOccurrence rdf:type owl:Class ;
                                rdfs:subClassOf [ rdf:type owl:Restriction ;
                                                  owl:onProperty :occurrenceOf ;
                                                  owl:someValuesFrom owl:Thing
                                                ] ,
                                                [ rdf:type owl:Restriction ;
                                                  owl:onProperty :source ;
                                                  owl:someValuesFrom owl:Thing
                                                ] ,
                                                [ rdf:type owl:Restriction ;
                                                  owl:onProperty :target ;
                                                  owl:someValuesFrom owl:Thing
                                                ] ,
                                                [ rdf:type owl:Restriction ;
                                                  owl:onProperty :occurrenceOf ;
                                                  owl:allValuesFrom :LinguisticPhenomenon
                                                ] ;
                                rdfs:comment "Occurrence of a linguistic phenomenon. Individuals of this class are the reified counterpart of assertions involving linguistic phenomena." ;
                                rdfs:label "Linguistic Phenomenon Occurence" .


#################################################################
#    Individuals
#################################################################

###  https://gallosiciliani.unict.it/ns/liph
<https://gallosiciliani.unict.it/ns/liph> rdf:type owl:NamedIndividual ;
                                          eurio:isResultOf :gallosiciliani2023Project .


###  https://gallosiciliani.unict.it/ns/liph#gallosiciliani2023Project
:gallosiciliani2023Project rdf:type owl:NamedIndividual ,
                                    eurio:Project ;
                           rdfs:comment "Research project “Contact-induced change and sociolinguistics: an experimental study on the Gallo-Italic dialects of Sicily\", founded by the European Union – Next Generation EU, Mission 4, Component 1, CUP J53D23017360001 - ID P2022YWS8T;" ;
                           rdfs:label "Contact-induced change and sociolinguistics: an experimental study on the Gallo-Italic dialects of Sicily" .


###  Generated by the OWL API (version 4.5.29.2024-05-13T12:11:03Z) https://github.com/owlcs/owlapi
