@prefix : <https://gallosiciliani.unict.it/ns/liph#> .
@prefix owl: <http://www.w3.org/2002/07/owl#> .
@prefix rdf: <http://www.w3.org/1999/02/22-rdf-syntax-ns#> .
@prefix xml: <http://www.w3.org/XML/1998/namespace> .
@prefix xsd: <http://www.w3.org/2001/XMLSchema#> .
@prefix rdfs: <http://www.w3.org/2000/01/rdf-schema#> .
@prefix vann: <http://purl.org/vocab/vann/> .
@prefix eurio: <http://data.europa.eu/s66#> .
@prefix dcterms: <http://purl.org/dc/terms/> .
@prefix ontolex: <https://www.w3.org/ns/lemon/ontolex#> .
@base <https://gallosiciliani.unict.it/ns/liph#> .

<https://gallosiciliani.unict.it/ns/liph> rdf:type owl:Ontology ;
                                           owl:versionIRI <https://gallosiciliani.unict.it/ns/liph/2.0.0> ;
                                           owl:imports <http://www.w3.org/ns/lemon/ontolex> ,
                                                       <https://gallosiciliani.unict.it/ns/projects> ;
                                           dcterms:contributor "Daniele Francesco Santamaria" ,
                                                               "Domenico Cantone" ,
                                                               "Marianna Nicolosi Asmundo" ,
                                                               "Salvatore Menza" ,
                                                               "Vincenzo Nicolò Di Caro" ;
                                           dcterms:created "2024-08-08"^^xsd:date ;
                                           dcterms:creator "Cristiano Longo" ;
                                           dcterms:description """The Linguistic Phenomena Ontology is an Ontolex-lemon extension devoted to represent linguistic phenomena.  We denote as linguistic phenomena those kinds of phenomena which cause modifications of language expressions. In general, a linguistic phenomenon occurs by turning a parent expression into a target expression in the language under consideration, where the parent expression may have been inherited from the parent language, or it may have been borrowed from a foreign language.

Generic linguistic phenomena are represented by the class LinguisticPhenomenon.
In addition, the ontology provides the FiniteStateLinguisticPhenomenon class and the datatype properties matchingPattern and replaceWith to describe a linguistic phenomenon operationally in a machine-actionable way.

Linguistic phenomena occurrences can be modeled throught the LinguisticPhenomenonOccurrence class and the properties source and target.

Finally, the derives property is used to model linguistic phenomena occurrences chains.

This work has been created in the scope of the project PRIN 2022 PNRR “Contact-induced change and sociolinguistics: an experimental study on the Gallo-Italic dialects of Sicily\", founded by the European Union – Next Generation EU, Mission 4, Component 1, CUP J53D23017360001 - ID P2022YWS8T."""@en ;
                                           dcterms:license <https://creativecommons.org/licenses/by/4.0/> ;
                                           dcterms:modified "2025-07-15" ;
                                           dcterms:title "The Linguistic Phenomena Ontology (LiPh)"@en ;
                                           vann:preferredNamespacePrefix "liph" ;
                                           vann:preferredNamespaceUri "https://gallosiciliani.unict.it/ns/liph#" ;
                                           rdfs:comment """The Linguistic Phenomena Ontology is an Ontolex-lemon extension devoted to represent linguistic phenomena.  We denote as linguistic phenomena those kinds of phenomena which cause modifications of language expressions. In general, a linguistic phenomenon occurs by turning a parent expression into a target expression in the language under consideration, where the parent expression may have been inherited from the parent language, or it may have been borrowed from a foreign language.

In addition, the ontology provides the regex and replacement properties to describe a linguistic phenomenon operatioanally in a machine-actionable way."""@en ;
                                           rdfs:label "The Linguistic Phenomena Ontology (LiPh)"@en ;
                                           owl:priorVersion "1.2.0" ;
                                           owl:versionInfo "2.0.0" .

#################################################################
#    Annotation properties
#################################################################

###  http://data.europa.eu/s66#isResultOf
eurio:isResultOf rdf:type owl:AnnotationProperty .


###  http://purl.org/dc/terms/contributor
dcterms:contributor rdf:type owl:AnnotationProperty .


###  http://purl.org/dc/terms/created
dcterms:created rdf:type owl:AnnotationProperty .


###  http://purl.org/dc/terms/creator
dcterms:creator rdf:type owl:AnnotationProperty .


###  http://purl.org/dc/terms/description
dcterms:description rdf:type owl:AnnotationProperty .


###  http://purl.org/dc/terms/license
dcterms:license rdf:type owl:AnnotationProperty .


###  http://purl.org/dc/terms/title
dcterms:title rdf:type owl:AnnotationProperty .


###  http://purl.org/vocab/vann/preferredNamespacePrefix
vann:preferredNamespacePrefix rdf:type owl:AnnotationProperty .


###  https://gallosiciliani.unict.it/ns/liph#regex
:regex rdf:type owl:AnnotationProperty ;
       rdfs:comment "Used in conjuction with replacement, it allows one to provide an operational description of a linguistic phenomenon. In particular, regex represent the regular expression which recognizes the parts of the parent strings which may be affected by the phenomenon." ;
       rdfs:label "Regular expression pattern" ;
       owl:deprecated "true"^^xsd:boolean ;
       rdfs:range xsd:string ;
       rdfs:domain :linguisticPhenomenon .


###  https://gallosiciliani.unict.it/ns/liph#replacement
:replacement rdf:type owl:AnnotationProperty ;
             rdfs:comment "Used in conjuction with regex, it allows one to provide an operational description of a linguistic phenomenon. In particular, this property define  how parts of the language expression matching the regex have to be replaced. Replacements may contain references to capturing groups defined in regex." ;
             rdfs:label "replacement" ;
             owl:deprecated "true"^^xsd:boolean ;
             rdfs:range xsd:string ;
             rdfs:domain :linguisticPhenomenon .


#################################################################
#    Object Properties
#################################################################

###  https://gallosiciliani.unict.it/ns/liph#derives
:derives rdf:type owl:ObjectProperty ,
                  owl:TransitiveProperty ,
                  owl:ReflexiveProperty ;
         owl:propertyChainAxiom ( [ owl:inverseOf :source
                                  ]
                                  :target
                                ) ;
         rdfs:comment "A derivation is a chain of linguistic phenomena occurrences, may be zero-lenght, which turned the subject lexical expression into the object one." ;
         rdfs:label "derives" .


###  https://gallosiciliani.unict.it/ns/liph#linguisticPhenomenon
:linguisticPhenomenon rdf:type owl:ObjectProperty ,
                               owl:TransitiveProperty ,
                               owl:ReflexiveProperty ;
                      rdfs:comment "An hypothetical change in the morphology or pronunciation of a language expression. Usually, a procedural description of such a phenomenon can be provided (for example \"replace t with d\"). A linguistic phenomenon can generate several resulting expressions, for example if applied to different parts of source ones." ;
                      rdfs:label "linguistic phenomenon" ;
                      owl:deprecated "true"^^xsd:boolean .


###  https://gallosiciliani.unict.it/ns/liph#occurrenceOf
:occurrenceOf rdf:type owl:ObjectProperty ,
                       owl:FunctionalProperty ;
              rdfs:comment "Denotes that an individual is an occurrence of a specific linguistic phenomenon." ;
              rdfs:label "occurrenceOf" .


###  https://gallosiciliani.unict.it/ns/liph#source
:source rdf:type owl:ObjectProperty ,
                 owl:FunctionalProperty ;
        rdfs:comment "The source lexical object, modified by the linguistic phenomenon." ;
        rdfs:label "source" .


###  https://gallosiciliani.unict.it/ns/liph#target
:target rdf:type owl:ObjectProperty ,
                 owl:FunctionalProperty ;
        rdfs:comment "How a source lexical object has been modified by the linguistic phenomenon." ;
        rdfs:label "target" .


#################################################################
#    Data properties
#################################################################

###  http://www.w3.org/ns/lemon/ontolex#writtenRep
<http://www.w3.org/ns/lemon/ontolex#writtenRep> rdfs:subPropertyOf :writtenRep .


###  https://gallosiciliani.unict.it/ns/liph#matchingPattern
:matchingPattern rdf:type owl:DatatypeProperty ,
                          owl:FunctionalProperty ;
                 rdfs:domain :FiniteStateLinguisticPhenomenon ;
                 rdfs:range xsd:string ;
                 rdfs:comment "A regular expression indicating the parts of a lexical expression which are subject to be replaced" ;
                 rdfs:label "matchingPattern" .


###  https://gallosiciliani.unict.it/ns/liph#replaceWith
:replaceWith rdf:type owl:DatatypeProperty ,
                      owl:FunctionalProperty ;
             rdfs:domain :FiniteStateLinguisticPhenomenon ;
             rdfs:range xsd:string ;
             rdfs:comment "How the matched parts of a lexical expression have to be replaced," ;
             rdfs:label "replaceWith" .


###  https://gallosiciliani.unict.it/ns/liph#writtenRep
:writtenRep rdf:type owl:DatatypeProperty ;
            rdfs:range rdf:langString ;
            rdfs:comment "A generalization of the writtenRep property of OntoLex." ;
            rdfs:label "writtenRep" .


#################################################################
#    Classes
#################################################################

###  http://www.w3.org/ns/lemon/ontolex#Form
<http://www.w3.org/ns/lemon/ontolex#Form> rdfs:subClassOf :LexicalObject .


###  https://gallosiciliani.unict.it/ns/liph#FiniteStateLinguisticPhenomenon
:FiniteStateLinguisticPhenomenon rdf:type owl:Class ;
                                 rdfs:subClassOf :LinguisticPhenomenon ,
                                                 [ rdf:type owl:Restriction ;
                                                   owl:onProperty :matchingPattern ;
                                                   owl:someValuesFrom xsd:string
                                                 ] ,
                                                 [ rdf:type owl:Restriction ;
                                                   owl:onProperty :replaceWith ;
                                                   owl:someValuesFrom xsd:string
                                                 ] ;
                                 rdfs:comment "An executable phenomenon described in terms of regular relations, using the data-properties matchingPattern and replaceWith." ;
                                 rdfs:label "FiniteStateLinguisticPhenomenon" .


###  https://gallosiciliani.unict.it/ns/liph#LexicalObject
:LexicalObject rdf:type owl:Class ;
               rdfs:subClassOf [ rdf:type owl:Restriction ;
                                 owl:onProperty :derives ;
                                 owl:allValuesFrom :LexicalObject
                               ] ,
                               [ rdf:type owl:Restriction ;
                                 owl:onProperty :writtenRep ;
                                 owl:someValuesFrom rdf:langString
                               ] ;
               owl:disjointWith :LinguisticPhenomenon ,
                                :LinguisticPhenomenonOccurrence ;
               rdfs:comment "A generic object representing a lexical expression someway involved in a lexical process." ;
               rdfs:label "LexicalObject" .


###  https://gallosiciliani.unict.it/ns/liph#LinguisticPhenomenon
:LinguisticPhenomenon rdf:type owl:Class ;
                      owl:disjointWith :LinguisticPhenomenonOccurrence ;
                      rdfs:comment "A phenomenon that change lexical expressions. Our linguistic phenomena are relations over orthographical forms. We don't exclude that this class could be used also for other kinds of phenomena." ;
                      rdfs:label "LinguisticPhenomenon" .


###  https://gallosiciliani.unict.it/ns/liph#LinguisticPhenomenonOccurrence
:LinguisticPhenomenonOccurrence rdf:type owl:Class ;
                                rdfs:subClassOf [ rdf:type owl:Restriction ;
                                                  owl:onProperty :occurrenceOf ;
                                                  owl:someValuesFrom owl:Thing
                                                ] ,
                                                [ rdf:type owl:Restriction ;
                                                  owl:onProperty :source ;
                                                  owl:someValuesFrom owl:Thing
                                                ] ,
                                                [ rdf:type owl:Restriction ;
                                                  owl:onProperty :target ;
                                                  owl:someValuesFrom owl:Thing
                                                ] ,
                                                [ rdf:type owl:Restriction ;
                                                  owl:onProperty :occurrenceOf ;
                                                  owl:allValuesFrom :LinguisticPhenomenon
                                                ] ;
                                rdfs:comment "An occurrence of a linguistic phenomenon. A linguistic phenomenon occurs when an expression from a source language (indicated with the source property) is transformed into one in a recipient language (indicated with the target property). Individuals of this class are the reified counterpart of assertions involving linguistic phenomena." ;
                                rdfs:label "LinguisticPhenomenonOccurence" .


#################################################################
#    Individuals
#################################################################

###  https://gallosiciliani.unict.it/ns/liph
<https://gallosiciliani.unict.it/ns/liph> eurio:isResultOf <https://gallosiciliani.unict.it/ns/projects/gallosiciliani2023Project> .


###  Generated by the OWL API (version 4.5.29.2024-05-13T12:11:03Z) https://github.com/owlcs/owlapi
