@prefix : <https://gallosiciliani.unict.it/ns/gs-features#> .
@prefix lp: <https://gallosiciliani.unict.it/ns/lp#> .
@prefix owl: <http://www.w3.org/2002/07/owl#> .
@prefix rdf: <http://www.w3.org/1999/02/22-rdf-syntax-ns#> .
@prefix xml: <http://www.w3.org/XML/1998/namespace> .
@prefix xsd: <http://www.w3.org/2001/XMLSchema#> .
@prefix rdfs: <http://www.w3.org/2000/01/rdf-schema#> .
@base <https://gallosiciliani.unict.it/ns/gs-features#> .

<https://gallosiciliani.unict.it/ns/gs-features> rdf:type owl:Ontology ;
                                                    owl:imports <https://gallosiciliani.unict.it/ns/lp> ;
                                                    rdfs:comment "Linguistic phenomena characterizing Gallo-Italian varieties spoken in Sicily." ;
                                                    rdfs:label "Gallo-Sicilian features" .

#################################################################
#    Object Properties
#################################################################

###  https://gallosiciliani.unict.it/ns/galloSicilian#nicosiaFeature
:nicosiaFeature rdf:type owl:ObjectProperty ;
                rdfs:subPropertyOf lp:linguisticPhenomenon ;
                rdfs:comment "A linguistic phenomena recurring in the language spoken in Novara di Sicilia." .


###  https://gallosiciliani.unict.it/ns/galloSicilian#northernItalyFeature
:northernItalyFeature rdf:type owl:ObjectProperty ;
                      rdfs:subPropertyOf lp:linguisticPhenomenon ;
                      rdfs:comment "A linguistic phenomenon typical of languages of northern Italy." .


###  https://gallosiciliani.unict.it/ns/galloSicilian#novaraDiSiciliaFeature
:novaraDiSiciliaFeature rdf:type owl:ObjectProperty ;
                        rdfs:subPropertyOf lp:linguisticPhenomenon ;
                        rdfs:comment "A linguistic phenomena recurring in the language spoken in Novara di Sicilia." .


###  https://gallosiciliani.unict.it/ns/galloSicilian#sanFratelloFeature
:sanFratelloFeature rdf:type owl:ObjectProperty ;
                    rdfs:subPropertyOf lp:linguisticPhenomenon ;
                    rdfs:comment "A linguistic phenomena recurring in the language spoken in the town of San Fratello, in Sicily." .


###  https://gallosiciliani.unict.it/ns/galloSicilian#southernItalyFeature
:southernItalyFeature rdf:type owl:ObjectProperty ;
                      rdfs:subPropertyOf lp:linguisticPhenomenon ;
                      rdfs:comment "A linguistic phenomenon typical of languages of southern Italy." .


###  https://gallosiciliani.unict.it/ns/galloSicilian#sperlingaFeature
:sperlingaFeature rdf:type owl:ObjectProperty ;
                  rdfs:subPropertyOf lp:linguisticPhenomenon ;
                  rdfs:comment "A linguistic phenomena recurring in the language spoken in Sperlinga, in Sicily." .


###  Generated by the OWL API (version 4.5.26.2023-07-17T20:34:13Z) https://github.com/owlcs/owlapi
